lib_misc/NullOrVarray.fst
@@ -1,0 +1,42 @@
+module NullOrVarray
+
+open Steel.Effect.Atomic
+open Steel.Effect
+open Steel.Reference
+module SM = Steel.Memory
+
+module A = Steel.Array
+
+open SteelOptUtils
+
+let array = Steel.ST.Array.array
+
+let null_or_varray (#a:Type) (r:array a)
+  : vprop
+  = c2 #(Seq.lseq a (A.length r))
+    (not (A.is_null r)) (A.varray r)
+
+let null_or_varray_t (#a: Type) (r:array a)
+  : Lemma
+  (t_of (null_or_varray #a r) == option (Seq.lseq a (A.length r)))
+  = ()
+
+noextract inline_for_extraction
+let intro_null_null_or_varray (#a: Type)
+  : Steel (array a)
+  emp
+  (fun r -> null_or_varray r)
+  (requires fun _ -> True)
+  (ensures fun _ r _ -> A.is_null r)
+  =
+  sladmit ();
+  return (A.null #a)
+
+let elim_null_null_or_varray (#opened:_) (#a: Type) (r: array a)
+  : SteelGhost unit opened
+  (null_or_varray r)
+  (fun _ -> emp)
+  (requires fun _ -> A.is_null r)
+  (ensures fun _ _ _ -> True)
+  =
+  sladmit ()
