src/Mman.fst
@@ -22,17 +22,31 @@ assume val mmap_init
       A.asel ptr h1 == Seq.create (US.v size) U8.zero
     )
 
+open NullOrVarray
+
+open Utils2
+
 //noextract
 assume val mmap_noinit
   (size: US.t)
   : Steel (array U8.t)
     emp
-    (fun ptr -> A.varray ptr)
+    (fun ptr -> null_or_varray ptr)
     (requires fun _ -> True)
     (ensures fun _ ptr h1 ->
-      A.length ptr == US.v size /\
-      A.is_full_array ptr /\
-      A.asel ptr h1 == Seq.create (US.v size) U8.zero
+      null_or_varray_t ptr;
+      let s
+        : normal (t_of (null_or_varray #U8.t ptr))
+        = h1 (null_or_varray ptr) in
+      let s
+        : option (Seq.lseq U8.t (A.length ptr))
+        = s in
+      not (A.is_null ptr) -> (
+        A.length ptr == US.v size /\
+        A.is_full_array ptr /\
+        Some? s /\
+        zf_u8 (Some?.v s)
+      )
     )
 
 //noextract
